---
date: 2021-06-25T17:37
---


# Data Analysis : Model Comparison Approach

Main issue is minimizing the residuals, or error. 

$$ DATA = MODEL + ERROR $$

Assuming that you have two models, a compact model (C) and an augmented model (A), *proportional reduction in error* (PRE) is calculated, 

$$PRE = \frac{ERROR(C) - ERROR(A)}{ERROR(C)}$$

Model A includes all the parameters of Model C plus an additional parameter.

Model C corresponds to the *null hypothesis* and Model A corresponds to the alternative hypothesis.


$Y_i$ : $i$th observation from $DATA$.

$\hat{Y_i}$ : Model's prediction of the $i$th observation

$X$ : gives information about each observation

$X_{ij}$ : $j$th predictor variable for the $i$th observation.

$\beta$ : true parameter

$\epsilon_{i}$ : Error 

$Y_i =  \beta_0 + \epsilon_{i}$ never know true parameter and error.

$e_i = Y_i - \hat{Y_i}$

$$MSE = \frac{SSE}{n-p}  = \frac{\sum_{i=1}^{n} (Y_i - \bar{Y}) ^ 2}{n-p}$$


$$ SSR = SSE(C) - SSE(A) $$



$$ F  = \frac{PRE/(PA - PC)}{(1-PRE)/(n - PA)} $$

Numerator indicates the average proportional reduction in error per parameter added, and the demoninator gives us the average proportioanl reduction in error that could be obtained by adding all possible remaining parameters.

The alternative formula for $F$ is:

$$ F = \frac{SSR/(PA - PC)}{SSE(A)/(n - PA)} = \frac{MSR}{MSE}$$



Unbiased estimate of $$\eta^2 = 1 - (1 - PRE)\left[\frac{n-PC}{n-PA}\right]$$


## Confidence Intervals

$$b_0 \pm \sqrt{\frac{F_{crit;1,n-1;a}MSE}{n}}$$

A *confidence interval* simply consists of all those possible values of a parameter that, when used as a hypothesis for Model C, would not cause us to reject Model C.

Confidence intervals are useful for describing post hoc the acutal statistical power achieved in terms of the precision of the parameter estimates. 


## Equivalence to the t-test

$$ t_{n-1} = \frac{\sqrt{n}(\bar{Y} - B_0)}{s} $$

$n$ : number of observations

$Y$ : calculated mean

$B_0$ : value specified by the null hypothesis

$$ F_{1, n-1} = t_{n-1}^2$$


*Proof* :

$$\begin{align}F_{1,n-1} &= \frac{PRE/1}{(1-PRE)/(n-1)}\tag{1}\\1-PRE &= 1 - \frac{SSR}{SSE(C)} = \frac{SSE(C)-SSR}{SSE(C)} = \frac{SSE(A)}{SSE(C)}\tag{2}\\ F_{1,n-1} &= \frac{SSR/SSE(C)}{[SSE(A)/SSE(C)]/(n-1)} = \frac{SSR}{SSE(A)/(n-1)}\tag{3} \\  F_{1,n-1} &= \frac{n (B_0 - \bar{Y})^2}{s^2}\tag{4}\\ \sqrt{F_{1,n-1}} &= t_{n-1} = \frac{\sqrt{n}(\bar{Y} - B_0)}{s}\tag{5}\end{align}$$

